abelian groups by generators and relations

src/Categories.v
@@ -792,9 +792,7 @@ Module Monoid.
     (** eta expansion principle for words *)
     Fixpoint reassemble {X I} (R:I->reln X) (v:wordop X) : evalword (wordop X) v == v.
     Proof. intros ? ? ? [|x|v w]. { reflexivity. } { reflexivity. }
-           { simpl. assert (p := !reassemble _ _ R v). destruct p.
-                    assert (q := !reassemble _ _ R w). destruct q.
-                    reflexivity. } Qed.
+           { exact (aptwice word_op (reassemble _ _ R v) (reassemble _ _ R w)). } Qed.
     (** ** adequate relations over R *)
     Record AdequateRelation {X I} (R:I->reln X) (r : hrel (word X)) := 
       make_AdequateRelation {
@@ -829,8 +827,7 @@ Module Monoid.
            { intros ? r ra. apply base. exact ra. }
            { intros ? r ra. apply (reflex R). exact ra. }
            { intros ? ? p r ra. apply (symm R). exact ra. exact (p r ra). }
-           { intros ? ? ? p q r ra. apply (trans R) with (v:=v).
-             exact ra. exact (p r ra). exact (q r ra). }
+           { exact (fun u v w p q r ra => trans R r ra u v w (p r ra) (q r ra)). }
            { intros ? ? ? p r ra. apply (left_compat R). exact ra. exact (p r ra). }
            { intros ? ? ? p r ra. apply (right_compat R). exact ra. exact (p r ra). }
            { intros ? r ra. apply (left_unit R). exact ra. }
@@ -1076,6 +1073,7 @@ End Group.
 Module AbelianGroup.
   Require Import Foundations.hlevel2.algebra1b.
   Local Notation Hom := monoidfun.
+  Local Notation "x * y" := ( op x y ). 
   Local Notation "g ∘ f" := (monoidfuncomp f g) (at level 50, only parsing).
   Definition commax (G:abgr) := pr2 (pr2 G).
   Definition zero : abgr.
@@ -1085,6 +1083,324 @@ Module AbelianGroup.
   Definition Z : abgr := hzaddabgr.
   Module Presentation.
     (** * abelian groups by generators and relations *)
+    (** This code is derived from the code in the module Monoid.Presentation.
+
+        Reduce the duplication later, if possible. *)
+    Inductive word X : Type :=
+      | word_unit : word X
+      | word_gen : X -> word X 
+      | word_inv : word X -> word X 
+      | word_op : word X -> word X -> word X.
+    Arguments word_unit {X}.
+    Arguments word_gen {X} x.
+    Arguments word_inv {X} w.
+    Arguments word_op {X} v w.
+    Record reln X := make_reln { lhs : word X; rhs : word X }.
+    Arguments lhs {X} r.
+    Arguments rhs {X} r.
+    Record MarkedPreAbelianGroup X := 
+      make_preAbelianGroup {
+          elem :> Type;
+          op0 : elem;
+          op1 : X -> elem;
+          op_inv : elem -> elem;
+          op2 : elem -> elem -> elem }.
+    Arguments elem {X} M : rename.
+    Arguments op0 {X M} : rename.
+    Arguments op1 {X M} x : rename.
+    Arguments op_inv {X M} x : rename.
+    Arguments op2 {X M} v w : rename.
+    Definition wordop X := make_preAbelianGroup X (word X) word_unit word_gen word_inv word_op.
+    Fixpoint evalword {X} (Y:MarkedPreAbelianGroup X) (w:word X) : elem Y.
+      intros ? Y [|x|w|v w]. { exact op0. } { exact (op1 x). }
+      { exact (op_inv (evalword X Y w)). }
+      { exact (op2 (evalword X Y v) (evalword X Y w)). } Defined.
+    Definition MarkedPreAbelianGroup_to_hrel {X} 
+               (M:MarkedPreAbelianGroup X) (is:isaset (elem M)) : 
+        hrel (word X) :=
+      fun v w => (evalword M v == evalword M w) ,, is _ _.
+    (** eta expansion principle for words *)
+    Fixpoint reassemble {X I} (R:I->reln X) (v:wordop X) : evalword (wordop X) v == v.
+    Proof. intros ? ? ? [|x|w|v w]. { reflexivity. } { reflexivity. }
+           { exact (ap word_inv (reassemble _ _ R w)). }
+           { exact (aptwice word_op (reassemble _ _ R v) (reassemble _ _ R w)). } Qed.
+    (** ** adequate relations over R *)
+    Record AdequateRelation {X I} (R:I->reln X) (r : hrel (word X)) := 
+      make_AdequateRelation {
+          base: forall i, r (lhs (R i)) (rhs (R i));
+          reflex : forall w, r w w;
+          symm : forall v w, r v w -> r w v;
+          trans : forall u v w, r u v -> r v w -> r u w;
+          left_compat : forall u v w, r v w -> r (word_op u v) (word_op u w);
+          right_compat: forall u v w, r u v -> r (word_op u w) (word_op v w);
+          left_unit : forall w, r (word_op word_unit w) w;
+          right_unit : forall w, r (word_op w word_unit) w;
+          assoc : forall u v w, r (word_op (word_op u v) w) (word_op u (word_op v w));
+          inverse_compat : forall v w, r v w -> r (word_inv v) (word_inv w);
+          left_inverse : forall w, r (word_op (word_inv w) w) word_unit;
+          right_inverse: forall w, r (word_op w (word_inv w)) word_unit;
+          comm : forall v w, r (word_op v w) (word_op w v)
+        }.
+    Arguments make_AdequateRelation {X I} R r _ _ _ _ _ _ _ _ _ _ _ _ _.
+    Arguments base {X I R r} _ _.
+    Definition adequacy_to_eqrel {X I} (R:I->reln X) (r : hrel (word X)) :
+      AdequateRelation R r -> eqrel (word X).
+    Proof. intros ? ? ? ? ra. exists r.
+           abstract ( split; [ split; [ exact (trans R r ra) | exact (reflex R r ra) ] |
+                               exact (symm R r ra)]). Defined.
+    (** ** the smallest adequate relation over R 
+           It is defined as the intersection of all the adequate relations.
+           Later we'll have to deal with the "resizing" to resolve issues
+           withe universes. *)
+    Definition smallestAdequateRelation0 {X I} (R:I->reln X) : hrel (word X).
+      intros ? ? ? v w.
+      exists (forall r: hrel (word X), AdequateRelation R r -> r v w).
+      abstract (apply impred; intro r; apply impred; intros _; apply propproperty).
+    Defined.
+    Lemma adequacy {X I} (R:I->reln X) : 
+      AdequateRelation R (smallestAdequateRelation0 R).
+    Proof. intros. refine (make_AdequateRelation R _ _ _ _ _ _ _ _ _ _ _ _ _ _).
+           { intros ? r ra. apply base. exact ra. }
+           { intros ? r ra. apply (reflex R). exact ra. }
+           { intros ? ? p r ra. apply (symm R). exact ra. exact (p r ra). }
+           { exact (fun u v w p q r ra => trans R r ra u v w (p r ra) (q r ra)). }
+           { intros ? ? ? p r ra. apply (left_compat R). exact ra. exact (p r ra). }
+           { intros ? ? ? p r ra. apply (right_compat R). exact ra. exact (p r ra). }
+           { intros ? r ra. apply (left_unit R). exact ra. }
+           { intros ? r ra. apply (right_unit R). exact ra. }
+           { exact (fun u v w r ra => assoc R r ra u v w). } 
+           { exact (fun v w p r ra => inverse_compat R r ra v w (p r ra)). }
+           { exact (fun w r ra => left_inverse R r ra w). } 
+           { exact (fun w r ra => right_inverse R r ra w). }
+           { exact (fun v w r ra => comm R r ra v w). }
+    Qed.
+    Definition smallestAdequateRelation {X I} (R:I->reln X) : eqrel (word X).
+      intros. exact (adequacy_to_eqrel R _ (adequacy R)). Defined.
+    (** *** the underlying set of the abelian group with generators X and relations R *)
+    Definition universalMarkedPreAbelianGroup0 {X I} (R:I->reln X) : hSet := 
+      setquotinset (smallestAdequateRelation R).
+    Lemma op_inv_compatibility {X I} (R:I->reln X) : 
+      iscomprelrelfun (smallestAdequateRelation R) (smallestAdequateRelation R) word_inv.
+    Proof. intros. intros v w p r ra. exact (inverse_compat R r ra v w (p r ra)). Qed.
+    Lemma op2_compatibility {X I} (R:I->reln X) : 
+      QuotientSet.iscomprelrelfun2
+        (smallestAdequateRelation R) (smallestAdequateRelation R) (smallestAdequateRelation R)
+        word_op.    
+    Proof. intros. split.
+      { intros x x' y p r ra. exact (right_compat R r ra x x' y (p r ra)). }
+      { intros x y y' p r ra. exact ( left_compat R r ra x y y' (p r ra)). } Qed.
+    (** *** the multiplication on on it *)
+    Definition univ_inverse {X I} (R:I->reln X) : 
+        universalMarkedPreAbelianGroup0 R -> universalMarkedPreAbelianGroup0 R.
+      intros ? ? ?.  refine (setquotfun _ _ word_inv _). apply op_inv_compatibility. Defined.
+    Definition univ_binop {X I} (R:I->reln X) : binop (universalMarkedPreAbelianGroup0 R).
+      intros. refine (QuotientSet.setquotfun2 word_op _). apply op2_compatibility. Defined.
+    Definition univ_setwithbinop {X I} (R:I->reln X) : setwithbinop
+               := setwithbinoppair (universalMarkedPreAbelianGroup0 R) (univ_binop R).
+    (** *** the universal pre-Abelian group *)
+    Definition universalMarkedPreAbelianGroup {X I} (R:I->reln X) : MarkedPreAbelianGroup X.
+      intros. refine (make_preAbelianGroup X (universalMarkedPreAbelianGroup0 R) _ _ _ _).
+      { exact (setquotpr _ word_unit). }
+      { exact (fun x => setquotpr _ (word_gen x)). }
+      { exact (univ_inverse _). }
+      { exact (univ_binop _). } Defined.
+    (** *** identities for the universal preabelian group *)
+    Lemma is_left_unit_univ_binop {X I} (R:I->reln X) : 
+      forall w : universalMarkedPreAbelianGroup0 R, ((univ_binop _) (setquotpr _ word_unit) w) == w.
+    Proof. intros ? ? ? w'. assert (lift := issurjsetquotpr (smallestAdequateRelation R)).
+      isaprop_goal ig. { apply setproperty. } 
+      apply (unsquash (lift w') ig); intros [w i]; destruct i; simpl.
+      exact (iscompsetquotpr (smallestAdequateRelation R) _ _ 
+                             (fun r ra => left_unit R r ra w)). Qed.
+    Lemma is_right_unit_univ_binop {X I} (R:I->reln X) : 
+      forall w : universalMarkedPreAbelianGroup0 R, ((univ_binop _) w (setquotpr _ word_unit)) == w.
+    Proof. intros ? ? ? w'. assert (lift := issurjsetquotpr (smallestAdequateRelation R)).
+      isaprop_goal ig. { apply setproperty. } 
+      apply (unsquash (lift w') ig); intros [w i]; destruct i; simpl.
+      exact (iscompsetquotpr (smallestAdequateRelation R) _ _ 
+                             (fun r ra => right_unit R r ra w)). Qed.
+    Lemma isassoc_univ_binop {X I} (R:I->reln X) : isassoc(univ_binop R).
+    Proof. intros. set (e := smallestAdequateRelation R). intros u' v' w'. 
+           isaprop_goal ig. { apply setproperty. } assert (lift := issurjsetquotpr e).
+ 	   apply (unsquash (lift u') ig); intros [u i]; destruct i; simpl.
+ 	   apply (unsquash (lift v') ig); intros [v j]; destruct j; simpl.
+ 	   apply (unsquash (lift w') ig); intros [w k]; destruct k; simpl.
+           exact (iscompsetquotpr e _ _ (fun r ra => assoc R r ra u v w)). Qed.
+    Lemma is_left_inverse_univ_binop {X I} (R:I->reln X) :
+      forall w:setquot (smallestAdequateRelation0 R),
+        univ_binop R (univ_inverse R w) w ==
+        setquotpr (smallestAdequateRelation R) word_unit.
+    Proof. intros. assert (lift := issurjsetquotpr (smallestAdequateRelation R)).
+      isaprop_goal ig. { apply setproperty. } 
+      apply (unsquash (lift w) ig); intros [v i]; destruct i; simpl.
+      exact (iscompsetquotpr (smallestAdequateRelation R) _ _ 
+                             (fun r ra => left_inverse R r ra v)). Qed.
+    Lemma is_right_inverse_univ_binop {X I} (R:I->reln X) :
+      forall w:setquot (smallestAdequateRelation0 R),
+        univ_binop R w (univ_inverse R w) ==
+        setquotpr (smallestAdequateRelation R) word_unit.
+    Proof. intros. assert (lift := issurjsetquotpr (smallestAdequateRelation R)).
+      isaprop_goal ig. { apply setproperty. } 
+      apply (unsquash (lift w) ig); intros [v i]; destruct i; simpl.
+      exact (iscompsetquotpr (smallestAdequateRelation R) _ _ 
+                             (fun r ra => right_inverse R r ra v)). Qed.
+    Lemma iscomm_univ_binop {X I} (R:I->reln X) : iscomm(univ_binop R).
+    Proof. intros. set (e := smallestAdequateRelation R). intros v' w'. 
+           isaprop_goal ig. { apply setproperty. } assert (lift := issurjsetquotpr e).
+ 	   apply (unsquash (lift v') ig); intros [v j]; destruct j; simpl.
+ 	   apply (unsquash (lift w') ig); intros [w k]; destruct k; simpl.
+           exact (iscompsetquotpr e _ _ (fun r ra => comm R r ra v w)). Qed.
+    (** *** adequacy under equality *)
+    Fixpoint reassemble_pr {X I} (R:I->reln X) (v:word X) : 
+      evalword (universalMarkedPreAbelianGroup R) v == setquotpr _ v.
+    Proof. intros ? ? ? [|x|w|v w]. { reflexivity. } { reflexivity. }
+           { simpl. assert (q := ! reassemble_pr _ _ R w). destruct q. reflexivity. }
+           { simpl. assert (p := ! reassemble_pr _ _ R v). destruct p.
+                    assert (q := ! reassemble_pr _ _ R w). destruct q.
+                    reflexivity. } Qed.
+    Lemma pr_eval_compat {X I} (R:I->reln X) (w:word X) :
+      setquotpr (smallestAdequateRelation R) (evalword (wordop X) w) 
+      == evalword (universalMarkedPreAbelianGroup R) w.
+    Proof. intros. destruct w as [|x|w|v w]. { reflexivity. } { reflexivity. } 
+      { exact (ap (setquotpr (smallestAdequateRelation R)) (reassemble R (word_inv w))
+             @ !reassemble_pr R (word_inv w)). }
+      { assert (p := !reassemble R (word_op v w)). destruct p. 
+        exact (!reassemble_pr R (word_op v w)). } Qed.
+    (** *** abelian groupss over X modulo R *)
+    Definition toMarkedPreAbelianGroup {X I} (R:I->reln X) (M:abgr) (el:X->M) : 
+        MarkedPreAbelianGroup X.
+      intros. exact {| elem := M; op0 := unel _; op1 := el; op_inv := grinv _; op2 := op |}.
+    Defined.
+    Record MarkedAbelianGroup {X I} (R:I->reln X) := 
+      make_MarkedAbelianGroup {
+          m_base :> abgr;
+          m_mark : X -> m_base;
+          m_reln : forall i, evalword (toMarkedPreAbelianGroup R m_base m_mark) (lhs (R i)) ==
+                             evalword (toMarkedPreAbelianGroup R m_base m_mark) (rhs (R i)) }.
+    Arguments make_MarkedAbelianGroup {X I} R _ _ _.
+    Arguments m_base {X I R} _.
+    Arguments m_mark {X I R} _ x.
+    Definition toMarkedPreAbelianGroup' {X I} {R:I->reln X} (M:MarkedAbelianGroup R) : MarkedPreAbelianGroup X :=
+      toMarkedPreAbelianGroup R (m_base M) (m_mark M).
+    Definition evalwordMM {X I} {R:I->reln X} (M:MarkedAbelianGroup R) : word X -> M :=
+      evalword (toMarkedPreAbelianGroup' M).
+    Definition MarkedAbelianGroup_to_hrel {X I} {R:I->reln X} (M:MarkedAbelianGroup R) : hrel (word X) :=
+      fun v w  => eqset (evalwordMM M v) (evalwordMM M w).
+    Lemma abelian_group_adequacy {X I} (R:I->reln X) (M:MarkedAbelianGroup R) :
+      AdequateRelation R (MarkedAbelianGroup_to_hrel M).
+    Proof. intros. refine (make_AdequateRelation R _ _ _ _ _ _ _ _ _ _ _ _ _ _).
+           { exact (fun i => m_reln R M i). } { reflexivity. }
+           { intros ? ?. exact pathsinv0. } { intros ? ? ?. exact pathscomp0. }
+           { intros ? ? ? p. simpl in p; simpl. 
+             unfold evalwordMM,evalword in *. destruct p. reflexivity. }
+           { intros ? ? ? p. simpl in p; simpl. 
+             unfold evalwordMM,evalword in *. destruct p. reflexivity. }
+           { intros. apply lunax. } { intros. apply runax. } { intros. apply assocax. } 
+           { intros ? ? p. simpl in p; simpl.
+             unfold evalwordMM,evalword in *. destruct p. reflexivity. }
+           { intros. apply grlinvax. } { intros. apply grrinvax. } { intros. apply commax. }
+    Qed.
+    Record MarkedAbelianGroupMap {X I} {R:I->reln X} (M N:MarkedAbelianGroup R) :=
+      make_MarkedAbelianGroupMap {
+          map_base :> Hom M N;
+          map_mark : forall x, map_base (m_mark M x) == m_mark N x }.
+    Arguments map_base {X I R M N} m.
+    Arguments map_mark {X I R M N} m x.
+    Lemma MarkedAbelianGroupMapEquality {X I} {R:I->reln X} {M N:MarkedAbelianGroup R}
+          (f g:MarkedAbelianGroupMap M N) : map_base f == map_base g -> f == g.
+    Proof. intros ? ? ? ? ? ? ? j.
+           destruct f as [f ft], g as [g gt]; simpl in j. destruct j.
+           assert(k : ft == gt). { apply funextsec; intro x. apply setproperty. } destruct k. 
+           reflexivity. Qed.
+    Fixpoint MarkedAbelianGroupMap_compat {X I} {R:I->reln X}
+             {M N:MarkedAbelianGroup R} (f:MarkedAbelianGroupMap M N) (w:word X) :
+      map_base f (evalwordMM M w) == evalwordMM N w.
+    Proof. intros. destruct w as [|x|w|v w].
+           { exact (Monoid.unitproperty f). }
+           { exact (map_mark f x). }
+           { exact (monoidfuninvtoinv f (evalwordMM M w)
+                  @ ap (grinv N) (MarkedAbelianGroupMap_compat _ _ _ _ _ f w)). }
+           { exact (Monoid.multproperty f (evalwordMM M v) (evalwordMM M w)
+                    @ aptwice (fun r s => r * s) 
+                              (MarkedAbelianGroupMap_compat _ _ _ _ _ f v) 
+                              (MarkedAbelianGroupMap_compat _ _ _ _ _ f w)). } Qed.
+    Lemma MarkedAbelianGroupMap_compat2 {X I} {R:I->reln X} 
+             {M N:MarkedAbelianGroup R} (f g:MarkedAbelianGroupMap M N) (w:word X) :
+      map_base f (evalwordMM M w) == map_base g (evalwordMM M w).
+    Proof. intros. 
+           exact (MarkedAbelianGroupMap_compat f w @ !MarkedAbelianGroupMap_compat g w). Qed.
+    (** *** the universal marked abelian group over X modulo R *)
+    Definition universalMarkedAbelianGroup0 {X I} (R:I->reln X) : abgr.
+      intros. 
+      { exists (univ_setwithbinop R). split.
+        { refine (_,,_).
+          { split.
+            { exact (isassoc_univ_binop R). }
+            { exists (setquotpr _ word_unit). split. 
+              { exact (is_left_unit_univ_binop R). }
+              { exact (is_right_unit_univ_binop R). } } }
+          { refine (_,,_).
+            { exact (univ_inverse R). }
+            { split.
+              { exact (is_left_inverse_univ_binop R). }
+              { exact (is_right_inverse_univ_binop R). } } } }
+        { exact (iscomm_univ_binop R). } }
+    Defined.
+    Definition universalMarkedAbelianGroup1 {X I} (R:I->reln X) : MarkedPreAbelianGroup X :=
+      (toMarkedPreAbelianGroup R 
+                    (universalMarkedAbelianGroup0 R)
+                    (fun x : X => setquotpr (smallestAdequateRelation R) (word_gen x))). 
+    Lemma universalMarkedAbelianGroup2 {X I} (R:I->reln X) (w:word X) : 
+      setquotpr (smallestAdequateRelation R) w == evalword (universalMarkedAbelianGroup1 R) w.
+    Proof. intros.
+      exact (! (ap (setquotpr (smallestAdequateRelation R)) (reassemble R w))
+             @ pr_eval_compat R w). Qed.
+    Definition universalMarkedAbelianGroup3 {X I} (R:I->reln X) (i:I) : 
+      evalword (universalMarkedAbelianGroup1 R) (lhs (R i)) ==
+      evalword (universalMarkedAbelianGroup1 R) (rhs (R i)).
+    Proof. intros.
+           exact (! universalMarkedAbelianGroup2 R (lhs (R i))
+                  @ iscompsetquotpr (smallestAdequateRelation R) _ _ (fun r ra => base ra i)
+                  @ universalMarkedAbelianGroup2 R (rhs (R i))). Qed.
+    Definition universalMarkedAbelianGroup {X I} (R:I->reln X) : MarkedAbelianGroup R :=
+      make_MarkedAbelianGroup R (universalMarkedAbelianGroup0 R) 
+                  (fun x => setquotpr (smallestAdequateRelation R) (word_gen x)) 
+                  (universalMarkedAbelianGroup3 R).
+    Definition universality0 {X I} {R:I->reln X} (M:MarkedAbelianGroup R) : 
+      universalMarkedAbelianGroup0 R -> M.
+    Proof. intros ? ? ? ?. 
+      apply (setquotuniv _ _ (evalwordMM M)).
+      exact (fun _ _ r => r (MarkedAbelianGroup_to_hrel M) (abelian_group_adequacy R M)).
+    Defined.
+    Definition universality1 {X I} (R:I->reln X) 
+                             (M:MarkedAbelianGroup R) (v w:universalMarkedAbelianGroup0 R) :
+      universality0 M (v * w) == universality0 M v * universality0 M w.
+    Proof. intros.
+           assert (lift := issurjsetquotpr (smallestAdequateRelation R)).
+           isaprop_goal ig. { apply setproperty. }
+           apply (unsquash (lift v) ig); intros [v' j]; destruct j; simpl.
+           apply (unsquash (lift w) ig); intros [w' k]; destruct k; simpl.
+           reflexivity. Qed.
+    Definition universality2 {X I} {R:I->reln X} (M:MarkedAbelianGroup R) : 
+      monoidfun (universalMarkedAbelianGroup R) M.
+    Proof. intros. exists (universality0 M).
+        split. { intros v w. apply universality1. } { reflexivity. } Defined.
+    (** * universality of the universal marked abelian group *)
+    Local Arguments pr1monoidfun {X Y} f x.
+    Theorem iscontrMarkedAbelianGroupMap {X I} {R:I->reln X} (M:MarkedAbelianGroup R) :
+          iscontr (MarkedAbelianGroupMap (universalMarkedAbelianGroup R) M).
+    Proof. intros. 
+      assert (g := make_MarkedAbelianGroupMap X I R 
+                             (universalMarkedAbelianGroup R) M 
+                             (universality2 M) (fun x => idpath _)).
+      exists g. intros f. apply MarkedAbelianGroupMapEquality.
+      apply Monoid.funEquality. apply funextfunax; intro v.
+      assert (lift := issurjsetquotpr (smallestAdequateRelation R)).
+      isaprop_goal ig. { apply setproperty. }
+      apply (unsquash (lift v) ig); intros [w j]; destruct j; simpl.
+      exact ((ap f (universalMarkedAbelianGroup2 R w)) 
+           @ MarkedAbelianGroupMap_compat2 f g w @ !(ap g (universalMarkedAbelianGroup2 R w))).
+    Qed.
   End Presentation.
   Module Product.
     Definition make {I} (X:I->abgr) : abgr.
